refactor(library/init/data): make sure `uint*` and `usize` are irreducible
Remark: this commit breaks the support for `uint*` and `usize` in the old VM.

library/init/data/uint.lean
@@ -7,78 +7,163 @@ prelude
 import init.data.fin.basic
 
 open nat
+
 def uint8_sz : nat := 65536
-def uint8 := fin uint8_sz
+structure uint8 :=
+(val : fin uint8_sz)
+
+def uint8.of_nat (n : nat) : uint8 := ⟨fin.of_nat n⟩
+def uint8.to_nat : uint8 → nat | ⟨a⟩ := a.val
+def uint8.add  : uint8 → uint8 → uint8 | ⟨a⟩ ⟨b⟩ := ⟨a + b⟩
+def uint8.sub  : uint8 → uint8 → uint8 | ⟨a⟩ ⟨b⟩ := ⟨a - b⟩
+def uint8.mul  : uint8 → uint8 → uint8 | ⟨a⟩ ⟨b⟩ := ⟨a * b⟩
+def uint8.div  : uint8 → uint8 → uint8 | ⟨a⟩ ⟨b⟩ := ⟨a / b⟩
+def uint8.mod  : uint8 → uint8 → uint8 | ⟨a⟩ ⟨b⟩ := ⟨a % b⟩
+def uint8.modn : uint8 → nat → uint8   | ⟨a⟩  b  := ⟨a %ₙ b⟩
+def uint8.lt   : uint8 → uint8 → Prop  | ⟨a⟩ ⟨b⟩ := a < b
+def uint8.le   : uint8 → uint8 → Prop  | ⟨a⟩ ⟨b⟩ := a ≤ b
+
+instance : has_zero uint8     := ⟨⟨fin.of_nat 0⟩⟩
+instance : has_one uint8      := ⟨⟨fin.of_nat 1⟩⟩
+instance : has_add uint8      := ⟨uint8.add⟩
+instance : has_sub uint8      := ⟨uint8.sub⟩
+instance : has_mul uint8      := ⟨uint8.mul⟩
+instance : has_mod uint8      := ⟨uint8.mod⟩
+instance : has_modn uint8     := ⟨uint8.modn⟩
+instance : has_div uint8      := ⟨uint8.div⟩
+instance : has_lt uint8       := ⟨uint8.lt⟩
+instance : has_le uint8       := ⟨uint8.le⟩
+instance : inhabited uint8    := ⟨0⟩
+
+def uint8.dec_eq : Π (a b : uint8), decidable (a = b)
+| ⟨a⟩ ⟨b⟩ := if h : a = b then is_true (h ▸ rfl) else is_false (λ h', uint8.no_confusion h' (λ h', absurd h' h))
+
+def uint8.dec_lt : Π (a b : uint8), decidable (a < b)
+| ⟨a⟩ ⟨b⟩ := infer_instance_as (decidable (a < b))
+
+def uint8.dec_le : Π (a b : uint8), decidable (a ≤ b)
+| ⟨a⟩ ⟨b⟩ := infer_instance_as (decidable (a ≤ b))
+
+instance : decidable_eq uint8 := {dec_eq := uint8.dec_eq}
+instance uint8.has_decidable_lt (a b : uint8) : decidable (a < b) := uint8.dec_lt a b
+instance uint8.has_decidable_le (a b : uint8) : decidable (a ≤ b) := uint8.dec_le a b
 
 def uint16_sz : nat := 65536
-def uint16 := fin uint16_sz
+structure uint16 :=
+(val : fin uint16_sz)
+
+def uint16.of_nat (n : nat) : uint16 := ⟨fin.of_nat n⟩
+def uint16.to_nat : uint16 → nat | ⟨a⟩ := a.val
+def uint16.add  : uint16 → uint16 → uint16 | ⟨a⟩ ⟨b⟩ := ⟨a + b⟩
+def uint16.sub  : uint16 → uint16 → uint16 | ⟨a⟩ ⟨b⟩ := ⟨a - b⟩
+def uint16.mul  : uint16 → uint16 → uint16 | ⟨a⟩ ⟨b⟩ := ⟨a * b⟩
+def uint16.div  : uint16 → uint16 → uint16 | ⟨a⟩ ⟨b⟩ := ⟨a / b⟩
+def uint16.mod  : uint16 → uint16 → uint16 | ⟨a⟩ ⟨b⟩ := ⟨a % b⟩
+def uint16.modn : uint16 → nat → uint16    | ⟨a⟩  b  := ⟨a %ₙ b⟩
+def uint16.lt   : uint16 → uint16 → Prop   | ⟨a⟩ ⟨b⟩ := a < b
+def uint16.le   : uint16 → uint16 → Prop   | ⟨a⟩ ⟨b⟩ := a ≤ b
+
+instance : has_zero uint16     := ⟨⟨fin.of_nat 0⟩⟩
+instance : has_one uint16      := ⟨⟨fin.of_nat 1⟩⟩
+instance : has_add uint16      := ⟨uint16.add⟩
+instance : has_sub uint16      := ⟨uint16.sub⟩
+instance : has_mul uint16      := ⟨uint16.mul⟩
+instance : has_mod uint16      := ⟨uint16.mod⟩
+instance : has_modn uint16     := ⟨uint16.modn⟩
+instance : has_div uint16      := ⟨uint16.div⟩
+instance : has_lt uint16       := ⟨uint16.lt⟩
+instance : has_le uint16       := ⟨uint16.le⟩
+instance : inhabited uint16    := ⟨0⟩
+
+def uint16.dec_eq : Π (a b : uint16), decidable (a = b)
+| ⟨a⟩ ⟨b⟩ := if h : a = b then is_true (h ▸ rfl) else is_false (λ h', uint16.no_confusion h' (λ h', absurd h' h))
+
+def uint16.dec_lt : Π (a b : uint16), decidable (a < b)
+| ⟨a⟩ ⟨b⟩ := infer_instance_as (decidable (a < b))
+
+def uint16.dec_le : Π (a b : uint16), decidable (a ≤ b)
+| ⟨a⟩ ⟨b⟩ := infer_instance_as (decidable (a ≤ b))
+
+instance : decidable_eq uint16 := {dec_eq := uint16.dec_eq}
+instance uint16.has_decidable_lt (a b : uint16) : decidable (a < b) := uint16.dec_lt a b
+instance uint16.has_decidable_le (a b : uint16) : decidable (a ≤ b) := uint16.dec_le a b
 
 def uint32_sz : nat := 4294967296
-def uint32 := fin uint32_sz
+structure uint32 :=
+(val : fin uint32_sz)
+
+def uint32.of_nat (n : nat) : uint32 := ⟨fin.of_nat n⟩
+def uint32.to_nat : uint32 → nat | ⟨a⟩ := a.val
+def uint32.add  : uint32 → uint32 → uint32 | ⟨a⟩ ⟨b⟩ := ⟨a + b⟩
+def uint32.sub  : uint32 → uint32 → uint32 | ⟨a⟩ ⟨b⟩ := ⟨a - b⟩
+def uint32.mul  : uint32 → uint32 → uint32 | ⟨a⟩ ⟨b⟩ := ⟨a * b⟩
+def uint32.div  : uint32 → uint32 → uint32 | ⟨a⟩ ⟨b⟩ := ⟨a / b⟩
+def uint32.mod  : uint32 → uint32 → uint32 | ⟨a⟩ ⟨b⟩ := ⟨a % b⟩
+def uint32.modn : uint32 → nat → uint32    | ⟨a⟩  b  := ⟨a %ₙ b⟩
+def uint32.lt   : uint32 → uint32 → Prop   | ⟨a⟩ ⟨b⟩ := a < b
+def uint32.le   : uint32 → uint32 → Prop   | ⟨a⟩ ⟨b⟩ := a ≤ b
+
+instance : has_zero uint32     := ⟨⟨fin.of_nat 0⟩⟩
+instance : has_one uint32      := ⟨⟨fin.of_nat 1⟩⟩
+instance : has_add uint32      := ⟨uint32.add⟩
+instance : has_sub uint32      := ⟨uint32.sub⟩
+instance : has_mul uint32      := ⟨uint32.mul⟩
+instance : has_mod uint32      := ⟨uint32.mod⟩
+instance : has_modn uint32     := ⟨uint32.modn⟩
+instance : has_div uint32      := ⟨uint32.div⟩
+instance : has_lt uint32       := ⟨uint32.lt⟩
+instance : has_le uint32       := ⟨uint32.le⟩
+instance : inhabited uint32    := ⟨0⟩
+
+def uint32.dec_eq : Π (a b : uint32), decidable (a = b)
+| ⟨a⟩ ⟨b⟩ := if h : a = b then is_true (h ▸ rfl) else is_false (λ h', uint32.no_confusion h' (λ h', absurd h' h))
+
+def uint32.dec_lt : Π (a b : uint32), decidable (a < b)
+| ⟨a⟩ ⟨b⟩ := infer_instance_as (decidable (a < b))
+
+def uint32.dec_le : Π (a b : uint32), decidable (a ≤ b)
+| ⟨a⟩ ⟨b⟩ := infer_instance_as (decidable (a ≤ b))
+
+instance : decidable_eq uint32 := {dec_eq := uint32.dec_eq}
+instance uint32.has_decidable_lt (a b : uint32) : decidable (a < b) := uint32.dec_lt a b
+instance uint32.has_decidable_le (a b : uint32) : decidable (a ≤ b) := uint32.dec_le a b
 
 def uint64_sz : nat := 18446744073709551616
-def uint64 := fin uint64_sz
+structure uint64 :=
+(val : fin uint64_sz)
 
-instance : decidable_eq uint8 := infer_instance_as (decidable_eq (fin uint8_sz))
-instance : decidable_eq uint16 := infer_instance_as (decidable_eq (fin uint16_sz))
-instance : decidable_eq uint32 := infer_instance_as (decidable_eq (fin uint32_sz))
-instance : decidable_eq uint64 := infer_instance_as (decidable_eq (fin uint64_sz))
+def uint64.of_nat (n : nat) : uint64 := ⟨fin.of_nat n⟩
+def uint64.to_nat : uint64 → nat | ⟨a⟩ := a.val
+def uint64.add  : uint64 → uint64 → uint64 | ⟨a⟩ ⟨b⟩ := ⟨a + b⟩
+def uint64.sub  : uint64 → uint64 → uint64 | ⟨a⟩ ⟨b⟩ := ⟨a - b⟩
+def uint64.mul  : uint64 → uint64 → uint64 | ⟨a⟩ ⟨b⟩ := ⟨a * b⟩
+def uint64.div  : uint64 → uint64 → uint64 | ⟨a⟩ ⟨b⟩ := ⟨a / b⟩
+def uint64.mod  : uint64 → uint64 → uint64 | ⟨a⟩ ⟨b⟩ := ⟨a % b⟩
+def uint64.modn : uint64 → nat → uint64    | ⟨a⟩  b  := ⟨a %ₙ b⟩
+def uint64.lt   : uint64 → uint64 → Prop   | ⟨a⟩ ⟨b⟩ := a < b
+def uint64.le   : uint64 → uint64 → Prop   | ⟨a⟩ ⟨b⟩ := a ≤ b
 
-instance : has_zero uint8  := ⟨fin.of_nat 0⟩
-instance : has_one uint8   := ⟨fin.of_nat 1⟩
-instance : has_add uint8   := ⟨fin.add⟩
-instance : has_sub uint8   := ⟨fin.sub⟩
-instance : has_mul uint8   := ⟨fin.mul⟩
-instance : has_mod uint8   := ⟨fin.mod⟩
-instance : has_modn uint8  := ⟨fin.modn⟩
-instance : has_div uint8   := ⟨fin.div⟩
-instance : has_lt uint8    := ⟨fin.lt⟩
-instance : has_le uint8    := ⟨fin.le⟩
-instance : inhabited uint8 := ⟨0⟩
+instance : has_zero uint64     := ⟨⟨fin.of_nat 0⟩⟩
+instance : has_one uint64      := ⟨⟨fin.of_nat 1⟩⟩
+instance : has_add uint64      := ⟨uint64.add⟩
+instance : has_sub uint64      := ⟨uint64.sub⟩
+instance : has_mul uint64      := ⟨uint64.mul⟩
+instance : has_mod uint64      := ⟨uint64.mod⟩
+instance : has_modn uint64     := ⟨uint64.modn⟩
+instance : has_div uint64      := ⟨uint64.div⟩
+instance : has_lt uint64       := ⟨uint64.lt⟩
+instance : has_le uint64       := ⟨uint64.le⟩
+instance : inhabited uint64    := ⟨0⟩
 
-instance : has_zero uint16  := ⟨fin.of_nat 0⟩
-instance : has_one uint16   := ⟨fin.of_nat 1⟩
-instance : has_add uint16   := ⟨fin.add⟩
-instance : has_sub uint16   := ⟨fin.sub⟩
-instance : has_mul uint16   := ⟨fin.mul⟩
-instance : has_mod uint16   := ⟨fin.mod⟩
-instance : has_modn uint16  := ⟨fin.modn⟩
-instance : has_div uint16   := ⟨fin.div⟩
-instance : has_lt uint16    := ⟨fin.lt⟩
-instance : has_le uint16    := ⟨fin.le⟩
-instance : inhabited uint16 := ⟨0⟩
+def uint64.dec_eq : Π (a b : uint64), decidable (a = b)
+| ⟨a⟩ ⟨b⟩ := if h : a = b then is_true (h ▸ rfl) else is_false (λ h', uint64.no_confusion h' (λ h', absurd h' h))
 
-instance : has_zero uint32  := ⟨fin.of_nat 0⟩
-instance : has_one uint32   := ⟨fin.of_nat 1⟩
-instance : has_add uint32   := ⟨fin.add⟩
-instance : has_sub uint32   := ⟨fin.sub⟩
-instance : has_mul uint32   := ⟨fin.mul⟩
-instance : has_mod uint32   := ⟨fin.mod⟩
-instance : has_modn uint32  := ⟨fin.modn⟩
-instance : has_div uint32   := ⟨fin.div⟩
-instance : has_lt uint32    := ⟨fin.lt⟩
-instance : has_le uint32    := ⟨fin.le⟩
-instance : inhabited uint32 := ⟨0⟩
+def uint64.dec_lt : Π (a b : uint64), decidable (a < b)
+| ⟨a⟩ ⟨b⟩ := infer_instance_as (decidable (a < b))
 
-instance : has_zero uint64  := ⟨fin.of_nat 0⟩
-instance : has_one uint64   := ⟨fin.of_nat 1⟩
-instance : has_add uint64   := ⟨fin.add⟩
-instance : has_sub uint64   := ⟨fin.sub⟩
-instance : has_mul uint64   := ⟨fin.mul⟩
-instance : has_mod uint64   := ⟨fin.mod⟩
-instance : has_modn uint64  := ⟨fin.modn⟩
-instance : has_div uint64   := ⟨fin.div⟩
-instance : has_lt uint64    := ⟨fin.lt⟩
-instance : has_le uint64    := ⟨fin.le⟩
-instance : inhabited uint64 := ⟨0⟩
+def uint64.dec_le : Π (a b : uint64), decidable (a ≤ b)
+| ⟨a⟩ ⟨b⟩ := infer_instance_as (decidable (a ≤ b))
 
-def uint8.of_nat (n : nat) : uint8 := fin.of_nat n
-def uint8.to_nat (u : uint8) : nat := u.val
-def uint16.of_nat (n : nat) : uint16 := fin.of_nat n
-def uint16.to_nat (u : uint16) : nat := u.val
-def uint32.of_nat (n : nat) : uint32 := fin.of_nat n
-def uint32.to_nat (u : uint32) : nat := u.val
-def uint64.of_nat (n : nat) : uint64 := fin.of_nat n
-def uint64.to_nat (u : uint64) : nat := u.val
-
-attribute [irreducible] uint8 uint16 uint32 uint64
+instance : decidable_eq uint64 := {dec_eq := uint64.dec_eq}
+instance uint64.has_decidable_lt (a b : uint64) : decidable (a < b) := uint64.dec_lt a b
+instance uint64.has_decidable_le (a b : uint64) : decidable (a ≤ b) := uint64.dec_le a b
